first_structure/Level.v
@@ -1,0 +1,872 @@
+Require Import Program.
+Require Import Coq.Arith.Bool_nat.
+
+Require Import Misc.
+Require Buffer.
+
+Record t (A : Set) : Set := makeLvl {
+  prefix  : Buffer.t A ;
+  suffix  : Buffer.t A
+}.
+
+Arguments makeLvl [A] _ _ .
+Arguments prefix [A] _.
+Arguments suffix [A] _.
+
+Definition color {A : Set} (lvl : t A) (is_last : bool) :=
+  if Buffer.dec_is_empty lvl.(suffix) then
+    if is_last then
+      Buffer.color lvl.(prefix)
+    else
+      Red
+  else if Buffer.dec_is_empty (prefix lvl) then
+    if is_last then
+      Buffer.color (suffix lvl)
+    else
+      Red
+  else
+    min_color (Buffer.color lvl.(prefix)) (Buffer.color lvl.(suffix)).
+
+Definition is_empty {A : Set} (lvl : t A) :=
+  Buffer.is_empty (prefix lvl) /\ Buffer.is_empty (suffix lvl).
+
+Definition dec_is_empty {A : Set} (lvl : t A) :
+  { is_empty lvl } + { ~ is_empty lvl }.
+  destruct lvl ; destruct prefix0, suffix0 ; firstorder.
+Defined.
+
+Program Definition push {A : Set} (x : A) (t : t A) (is_last : bool)
+  (proof : color t is_last <> Red \/ is_empty t) :=
+  if Buffer.dec_is_empty (prefix t) then
+    makeLvl (Buffer.push x (suffix t)) Buffer.Zero
+  else
+    makeLvl (Buffer.push x (prefix t)) (suffix t).
+
+Next Obligation.
+Proof.
+  destruct t0 ; compute in proof;
+  destruct (Buffer.dec_is_empty prefix0), (Buffer.dec_is_empty suffix0);
+  destruct prefix0, suffix0, is_last ; firstorder.
+Qed.
+
+Next Obligation.
+Proof.
+  destruct t0 ; compute in proof |- *;
+  destruct (Buffer.dec_is_empty prefix0), (Buffer.dec_is_empty suffix0);
+  destruct prefix0, suffix0, is_last ; firstorder;
+  left ; intro Color_mismatch ; discriminate Color_mismatch.
+Qed.
+
+Theorem red_push_iff_yellow :
+  forall A x is_last, forall t : t A,
+  forall p : color t is_last <> Red \/ is_empty t,
+    color (push x t is_last p) is_last = Red -> color t is_last <> Green.
+Proof.
+  intros.
+  destruct t0, is_last ; destruct prefix0, suffix0 ; compute in * ;
+  firstorder ; solve [
+    discriminate H | discriminate H0 |
+    (clear H ; destruct p as [ H1 | H1 ]  ; exfalso ; [ 
+      (apply H1 ; reflexivity) | (destruct H1 ; assumption)
+    ])
+  ].
+Qed.
+
+Definition empty (A : Set) := makeLvl (A := A) Buffer.Zero Buffer.Zero.
+
+Notation "x ≥ y" := (ge_dec x y) (at level 70, right associativity).
+
+Require Import Omega.
+
+Obligation Tactic := (program_simpl;
+    try (
+      (simpl in * |- *; apply Buffer.nonempty_length; omega)
+    || (left; congruence)
+    || (try split ; omega)
+    )).
+
+Program Definition two_buffer_case {A}
+  (lvli : t A)
+  (lvlSi : t (A * A))
+  (Colori : color lvli false = Red)
+  (last_Si : bool)
+  (ColorSi : color lvlSi last_Si<> Red)
+  (H : (Buffer.length (prefix lvlSi)) + (Buffer.length (suffix lvlSi)) >= 2)
+  : { li  : t A | color li false = Green } *
+    { lSi : t (A * A)
+        | (color lSi last_Si= Red -> color lvlSi last_Si<> Green \/ last_Si = true)
+    }
+:=
+  
+  let pairSi
+  : { p : Buffer.t (A * A) |
+      Buffer.color p <> Red /\
+      (Buffer.color p <> Green -> color lvlSi last_Si <> Green \/ last_Si = true)
+    } * 
+    { s : Buffer.t (A * A) |
+      Buffer.color s <> Red /\
+      (Buffer.color s <> Green -> color lvlSi last_Si <> Green \/ last_Si = true)
+    }
+  :=
+    match Buffer.dec_is_empty (prefix lvlSi), Buffer.dec_is_empty (suffix lvlSi) with
+    | left _, left _ => 
+        (* By H. *)
+        !
+    | left _, right _ =>
+        (* We have at least two elements in the suffix: 
+            we push the first of theses elements in the prefix. *)
+        let (p, Hp) := Buffer.pop (suffix lvlSi) in
+        let '(elt, buff) := p in
+        pair (Buffer.One elt) buff
+    | right _, left _ =>
+        (* Symmetric case. *)
+        let (p, Hp) := Buffer.eject (prefix lvlSi) in
+        let '(elt, buff) := p in
+        pair buff (Buffer.One elt)
+    | right _, right _ => 
+        (* None of the two buffers is empty. *)
+        (prefix lvlSi, suffix lvlSi)
+    end
+  in
+  let (pSi, sSi) := pairSi in
+  let pairP :
+    { b : Buffer.t A | Buffer.color b = Green } *
+    { b : Buffer.t (A * A)
+        | Buffer.color b = Red -> color lvlSi last_Si <> Green \/ last_Si = true }
+  :=
+    match Buffer.length (prefix lvli) ≥ 4 with 
+    | left _ =>
+      let (p, Hp) := Buffer.eject (prefix lvli) in
+      let '(elt1, buff1) := p in
+      let (p, Hp) := Buffer.eject buff1 in
+      let '(elt2, buff2) := p in
+      let (buff3, Hlol) := Buffer.push (elt2, elt1) pSi in
+      (buff2, buff3)
+    | right _ =>
+      match 1 ≥ Buffer.length (prefix lvli) with
+      | left _ =>
+        let (pair, HpSi) := Buffer.pop pSi in
+        let '(p, pSi) := pair in
+        let '(elt1, elt2) := p in
+        let (buff, Hbuff) := Buffer.inject elt1 (prefix lvli) in
+        let (buff2, Hbuff2) := Buffer.inject elt2 buff in
+        (buff2, pSi)
+      | right _ =>
+        (prefix lvli, pSi)
+      end
+    end
+  in
+  let pairS :
+    { b : Buffer.t A | Buffer.color b = Green } *
+    { b : Buffer.t (A * A)
+        | Buffer.color b = Red -> color lvlSi last_Si <> Green \/ last_Si = true }
+  :=
+    match (Buffer.length (suffix lvli)) ≥ 4 with
+    | left H =>
+      let (p, Hp) := Buffer.pop (suffix lvli) in
+      let '(elt1, buff) :=  p in
+      let (p, H) := Buffer.pop buff in
+      let '(elt2, buff) := p in
+      let (buff2, Hlol) := Buffer.inject (elt1, elt2) sSi in
+      (buff, buff2)
+    | right _ =>
+      match 1 ≥ (Buffer.length (suffix lvli)) with
+      | left _ =>
+        let (pair, HsSi) := Buffer.eject sSi in
+        let '(p, sSi) := pair in
+        let '(elt1, elt2) := p in
+        let (buff, Hbuff) := Buffer.push elt2 (suffix lvli) in
+        let (buff2, Hbuff2) := Buffer.push elt1 buff in
+        (buff2, sSi)
+      | right _ =>
+        (suffix lvli, sSi)
+      end
+    end
+  in
+  let (pi, pSi) := pairP in
+  let (si, sSi) := pairS in
+  (makeLvl pi si, makeLvl pSi sSi).
+
+Next Obligation.
+Proof.
+  assert (Buffer.length (prefix lvlSi) = 0) by (apply Buffer.empty_length; auto).
+  assert (Buffer.length (suffix lvlSi) = 0) by (apply Buffer.empty_length; auto).
+  omega.
+Qed.
+
+Next Obligation. 
+Proof. 
+  split ; [ discriminate | intro ].
+  assert (Hs: Buffer.length (prefix lvlSi) = 0) by (apply Buffer.empty_length; auto).
+  rewrite Hs in H; simpl in H.
+  assert (Buffer.length (suffix lvlSi) <= 5) by (apply Buffer.bounded_length).    
+  destruct lvlSi; destruct prefix0, suffix0, last_Si; simpl in * ; try solve [
+    omega |
+    contradiction |
+    (right ;reflexivity) |
+    (left ; compute ; discriminate) |
+    (compute in ColorSi ; discriminate ColorSi)
+  ].
+Qed.
+
+Next Obligation.
+Proof.
+  simpl in *.
+  assert (Hs: Buffer.length (prefix lvlSi) = 0) by (apply Buffer.empty_length; auto).
+  rewrite Hs in H; simpl in H.
+  assert (Buffer.length (suffix lvlSi) <= 5) by (apply Buffer.bounded_length).    
+  split.
+  - destruct t0 ; simpl in * ; discriminate || omega.
+  - intro.
+    destruct lvlSi ; destruct prefix0, suffix0, last_Si ; simpl in * ;
+    solve [
+      omega | (right ; reflexivity) | (left ; compute ; discriminate)
+    ].
+Qed.
+
+Next Obligation.
+Proof.
+  simpl in *.
+  assert (Hs: Buffer.length (suffix lvlSi) = 0) by (apply Buffer.empty_length; auto).
+  rewrite Hs in H; simpl in H.
+  assert (Buffer.length (prefix lvlSi) <= 5) by (apply Buffer.bounded_length).    
+  split.
+  - destruct t0 ; simpl in * ; discriminate || omega.
+  - intro.
+    destruct lvlSi ; destruct prefix0, suffix0, last_Si ; simpl in * ;
+    solve [
+      omega | (right ; reflexivity) | (left ; compute ; discriminate)
+    ].
+Qed.
+
+Next Obligation.
+Proof.
+  simpl in *.
+  split ; [ discriminate | intro ].
+  assert (Hs: Buffer.length (suffix lvlSi) = 0) by (apply Buffer.empty_length; auto).
+  rewrite Hs in H; simpl in H.
+  assert (Buffer.length (prefix lvlSi) <= 5) by (apply Buffer.bounded_length).    
+  destruct lvlSi ; destruct prefix0, suffix0, last_Si ; simpl in * ; solve [
+    omega |
+    (right ; reflexivity) |
+    (left ; compute ; discriminate)
+  ].
+Qed.
+
+Next Obligation.
+Proof.
+  destruct lvlSi; compute in ColorSi |- * .
+  destruct prefix0, suffix0, last_Si ; simpl in * ; solve [
+    auto with arith |
+    (split ; [ idtac | intro ; left ] ; intro F ; discriminate F)
+  ].
+Qed.
+
+Next Obligation.
+Proof.
+  destruct lvlSi; compute in ColorSi |- * ;
+  destruct prefix0, suffix0, last_Si ; simpl in * ; solve [
+    auto with arith |
+    (split ; [ idtac | intro ; left ] ; intro F ; discriminate F)
+  ].
+Qed.
+
+Next Obligation.
+Proof.
+  simpl in *.
+  assert (Hmax : Buffer.length (prefix lvli) <= 5) by apply Buffer.bounded_length.
+  destruct (Buffer.length (prefix lvli)) ; try omega.
+  destruct t0 ; simpl in Hp0 ; try omega ; simpl ; reflexivity.
+Qed.
+
+Next Obligation.
+Proof.
+  simpl in * ; apply o.
+  destruct buff3 ; simpl in * ; first [ omega | discriminate H0 | idtac ].
+  destruct pSi ; simpl in * ; omega || discriminate.
+Qed.
+
+Next Obligation.
+Proof.
+  destruct pSi ; simpl in n ; solve [
+    (contradict n ; reflexivity) |
+    (compute ; trivial)
+  ].
+Qed.
+
+Next Obligation.
+Proof.
+  destruct lvli; destruct prefix0; simpl ; solve [
+    (right ; trivial) |
+    (left ; discriminate)
+  ].
+Qed.
+
+Next Obligation.
+Proof.
+  simpl in * ; left.
+  destruct (Buffer.length (prefix lvli)).
+  + destruct buff ; simpl in Hbuff ; discriminate || discriminate Hbuff.
+  + assert (Hn : n0 = 0) by omega.
+    destruct buff ; simpl in Hbuff ; discriminate || (exfalso ; omega).
+Qed.
+
+Next Obligation.
+Proof.
+  simpl in *.
+  destruct (Buffer.length (prefix lvli)) ; try omega ;
+  rewrite Hbuff in Hbuff2 ;
+  destruct buff2 ; simpl in * ; try omega ; reflexivity.
+Qed.
+
+Next Obligation.
+Proof.
+  simpl in *; apply o.
+  destruct pSi, t0 ; simpl in * ; omega || discriminate.
+Qed.
+
+Next Obligation.
+Proof.
+  destruct (prefix lvli) ; simpl in * ; solve [ omega | reflexivity ].
+Qed.
+
+Next Obligation.
+Proof.
+  simpl in *.
+  assert (Hmax : Buffer.length (suffix lvli) <= 5) by apply Buffer.bounded_length.
+  destruct (Buffer.length (suffix lvli)) ; try omega.
+  destruct t0 ; simpl in H1 ; try omega ; simpl ; reflexivity.
+Qed.
+
+Next Obligation.
+Proof.
+  simpl in * ; apply o.
+  destruct sSi, buff2 ; simpl in * ; omega || discriminate.
+Qed.
+
+Next Obligation.
+Proof.
+  destruct sSi ; simpl in * ; solve [ (contradict n ; reflexivity) | auto ].
+Qed.
+
+Next Obligation.
+Proof.
+  destruct (suffix lvli) ; simpl in * ; solve [
+    omega |
+    (left ; discriminate) |
+    (right ; trivial)
+  ].
+Qed.
+
+Next Obligation.
+Proof.
+  left ; simpl in *.
+  destruct (Buffer.length (suffix lvli)), buff ; simpl in * ; omega || discriminate.
+Qed.
+
+Next Obligation.
+Proof.
+  simpl in *.
+  destruct (Buffer.length (prefix lvli)) ; try omega ;
+  rewrite Hbuff in Hbuff2 ;
+  destruct buff2 ; simpl in * ; try omega ; reflexivity.
+Qed.
+
+Next Obligation.
+Proof.
+  simpl in * ; apply o.
+  destruct t0, sSi ; simpl in * ; try (omega || discriminate H0).
+  discriminate.
+Qed.
+
+Next Obligation.
+Proof.
+  destruct (suffix lvli) ; simpl in * ; solve [ omega | reflexivity ].
+Qed.
+
+Next Obligation.
+Proof.
+  destruct pi, si ; simpl in H1, H3 ; first [
+    discriminate H3 | discriminate H1 | idtac
+  ] ; simpl ; reflexivity.
+Qed.
+
+Next Obligation.
+Proof.
+  destruct pSi0, sSi0 ; simpl in * ; try solve [
+    (compute in H0 ; discriminate H0) |
+    (apply H1 ; reflexivity) |
+    (apply H3 ; reflexivity)
+  ].
+Qed.
+
+(* A note on the hypotheses :
+  *   [ColorSi] assert that [lvlSi] might be empty. If that is the case, it
+  *   means that we just created it, implying that [lvli] was the bottom-most
+  *   level, and the conjunction of [Colori] and [Hi] tells us that one of its
+  *   buffers is full. *)
+Program Definition one_buffer_case {A}
+  (lvli : t A)
+  (lvlSi : t (A * A))
+  (is_lasti is_lastSi : bool)
+  (Colori : color lvli is_lasti = Red)
+  (ColorSi : color lvlSi is_lastSi <> Red \/ is_empty lvlSi)
+  (HSi : (Buffer.length (prefix lvlSi)) + (Buffer.length (suffix lvlSi)) <= 1)
+  (Hi : Buffer.length (prefix lvli) >= 2 \/ Buffer.length (suffix lvli) >= 2)
+  (LastLvl : is_empty lvlSi -> is_lasti = true)
+  (Triviality : is_lasti = true -> is_lastSi = true)
+: { l : t A | color l false = Green } * t (A * A)
+:=
+  let pSi_sig :
+    { b : Buffer.t (A * A) |
+      Buffer.length b <= 1 /\ (Buffer.length b = 0 -> is_lasti = true) }:=
+    match Buffer.length (suffix lvlSi) as len_suff with
+    | 0 => prefix lvlSi
+    | 1 => suffix lvlSi
+    | _ => ! (* by HSi *)
+    end
+  in
+  let (pSi, HpSi) := pSi_sig in
+  let pairP :
+    { b : Buffer.t A |
+      if Buffer.length (prefix lvli) ≥ 4
+        then 1 < Buffer.length b <= 3
+        else b = prefix lvli
+    } *
+    { b : Buffer.t (A * A) |
+      if Buffer.length (prefix lvli) ≥ 4
+        then 0 < Buffer.length b <= 2
+        else Buffer.length b <= 1 /\ (Buffer.length b = 0 -> is_lasti = true)
+    } :=
+    match Buffer.length (prefix lvli) ≥ 4 with 
+    | left _ =>
+      let (p, Hp) := Buffer.eject (prefix lvli) in
+      let '(elt1, buff1) := p in
+      let (p, Hp) := Buffer.eject buff1 in
+      let '(elt2, buff2) := p in
+      let (pSi_internal, HpSi_internal) := Buffer.push (elt2, elt1) pSi in
+      (buff2, pSi_internal)
+    | right _ =>
+      (* [prefix lvli] might contain less than two element, we want to pop
+        * from [pSi], but at that point it might still be empty. We need to
+        * push elements from [suffix lvli] (which by hypothesis contains more
+        * than 2 element) into it before we can replenish the prefix. *)
+      (prefix lvli, pSi)
+    end
+  in
+  let (pi, pSi) := pairP in
+  let pairSP : { b : Buffer.t A | Buffer.color b = Green } *
+    { b : Buffer.t (A * A) |
+      if Buffer.length (suffix lvli) ≥ 4
+        then 0 < Buffer.length b <= 3
+        else Buffer.length b <= 2
+              /\ (Buffer.length b = 0 ->
+                  Buffer.length (suffix lvli) <= 1 \/ is_lasti = true)
+    } :=
+    match (Buffer.length (suffix lvli)) ≥ 4 with
+    | left H =>
+      let (p, Hp) := Buffer.pop (suffix lvli) in
+      let '(elt1, buff) :=  p in
+      let (p, H) := Buffer.pop buff in
+      let '(elt2, buff) := p in
+      let (buff2, Hbuff2) := Buffer.inject (elt1, elt2) pSi in
+      (buff, buff2)
+    | right _ =>
+      match 1 ≥ (Buffer.length (suffix lvli)) with
+      | left _ =>
+        let (p, Hp) := Buffer.eject pSi in
+        let '((elt1, elt2), pSi) := p in
+        let (buff, Hbuff) := Buffer.push elt2 (suffix lvli) in
+        let (buff2, Hbuff2) := Buffer.push elt1 buff in
+        (buff2, pSi)
+      | right _ =>
+        (suffix lvli, pSi)
+      end
+    end
+  in
+  let (si, pSi) := pairSP in
+  let pairP2 : { b : Buffer.t A | Buffer.color b = Green }  * Buffer.t (A * A) :=
+    match 1 ≥ Buffer.length (prefix lvli) with
+    | left _ =>
+      let (p, Hp) := Buffer.pop pSi in
+      let '((elt1, elt2), pSi) := p in
+      let (buff, Hbuff) := Buffer.inject elt1 (prefix lvli) in
+      let (buff2, Hbuff2) := Buffer.inject elt2 buff in
+      (buff2, pSi)
+    | right _ =>
+      (pi, pSi)
+    end
+  in
+  let (pi, pSi) := pairP2 in
+  (makeLvl pi si, makeLvl pSi Buffer.Zero).
+
+Next Obligation.
+Proof.
+  split.
+  - omega.
+  - intro H ; apply LastLvl.
+    destruct lvlSi ; destruct prefix0, suffix0 ; simpl in *; firstorder.
+Qed.
+
+Next Obligation.
+Proof.
+  simpl in * ;
+  destruct pSi ; simpl in * ; try solve [
+    (right ; trivial) |
+    (left ; discriminate)
+  ] ;
+  omega.
+Qed.
+
+Next Obligation.
+Proof.
+  simpl in *.
+  assert (HB: Buffer.length (prefix lvli) <= 5) by apply Buffer.bounded_length.
+  destruct (Buffer.length (prefix lvli)) ; omega.
+Qed.
+
+Next Obligation.
+Proof.
+  destruct pSi0 ; simpl in * ; try solve [ (left ; discriminate) ] ; [
+    (right ; trivial) |
+    (destruct (Buffer.length (prefix lvli) ≥ 4) ; omega)
+  ].
+Qed.
+
+Next Obligation.
+Proof.
+  simpl in *.
+  assert (Hmax : Buffer.length (suffix lvli) <= 5) by apply Buffer.bounded_length.
+  destruct (Buffer.length (suffix lvli)) ; try omega.
+  injection Hp ; intro Hn ; rewrite Hn in H0 ; subst.
+  destruct t0 ; simpl in * ; try omega ; reflexivity.
+Qed.
+
+Next Obligation.
+Proof.
+  simpl in *.
+  destruct (Buffer.length (prefix lvli) ≥ 4) ; simpl in * ; omega.
+Qed.
+
+Next Obligation.
+Proof.
+  apply Buffer.nonempty_length.
+  destruct (Buffer.length (prefix lvli) ≥ 4) ; try omega.
+  destruct H1; inversion H1; try omega.
+  exfalso ; inversion H5.
+  apply H3 in H7.
+  destruct (Buffer.length (suffix lvli)) eqn:HLsi; try omega;
+  contradict Colori.
+  - destruct lvli; compute; simpl in *.
+    rewrite H7 ; simpl.
+    destruct prefix0, suffix0 ; intro ; simpl in * ; solve [
+      discriminate H6 | omega
+    ].
+  - assert (trivial : n0 = 0) by omega; subst.
+    destruct lvli; compute; simpl in *.
+    destruct prefix0, suffix0 ; intro ; simpl in * ; auto ;
+    try discriminate H2 ; omega.
+Qed. (* TODO: clean up *)
+
+Next Obligation.
+Proof.
+  inversion wildcard'0.
+  + left ; destruct (suffix lvli) ; simpl in H4 ; solve [
+      discriminate H4 |
+      (compute ; discriminate)
+    ].
+  + right ; apply Buffer.empty_length ; auto with arith.
+Qed.
+
+Next Obligation.
+Proof.
+  destruct (Buffer.length (suffix lvli));
+    [ idtac | (assert (n = 0) by omega ; subst) ] ;
+  left; destruct buff ; simpl in Hbuff ; discriminate || discriminate Hbuff.
+Qed.
+
+Next Obligation.
+Proof. 
+  simpl in *.
+  destruct (Buffer.length (suffix lvli)) ; try omega ;
+  destruct buff2 ; simpl in * ; try omega ; reflexivity.
+Qed.
+
+Next Obligation.
+Proof. 
+  simpl in * ; split; destruct (Buffer.length (prefix lvli) ≥ 4) ;
+  try left ; omega.
+Qed.
+
+Next Obligation.
+Proof.
+  simpl in *.
+  destruct (suffix lvli) ; simpl in * ; solve [ omega | reflexivity ].
+Qed.
+
+Next Obligation.
+Proof.
+  simpl in * ; split; destruct (Buffer.length (prefix lvli) ≥ 4) ; try omega.
+  intro HLpSi0 ; right.
+  destruct H1.
+  apply H3 ; apply HLpSi0.
+Qed.
+
+Next Obligation.
+Proof.
+  apply Buffer.nonempty_length.
+  destruct (Buffer.length (suffix lvli) ≥ 4) ; try omega.
+  destruct H1.
+  destruct (Buffer.length pSi1).
+  - assert (trivial : 0 = 0) by omega.
+    apply H5 in trivial.
+    destruct trivial.
+    + exfalso ; omega.
+    + contradict Colori.
+      destruct lvli ; compute; simpl in *; try rewrite H6;
+      destruct prefix0, suffix0 ; intro ; simpl in * ; omega || discriminate H7.
+  - auto with arith.
+Qed.
+
+Next Obligation.
+Proof.
+  destruct (prefix lvli) ; simpl in wildcard' ; solve [
+    (left ; compute ; discriminate) |
+    (right; simpl ; trivial) |
+    omega
+  ].
+Qed.
+
+Next Obligation.
+Proof.
+  left; destruct (Buffer.length pi); destruct buff ; solve [
+    (simpl in Hbuff ; omega) |
+    (compute ; intro C ; discriminate C)
+  ].
+Qed.
+
+Next Obligation.
+Proof.
+  destruct (prefix lvli) ; simpl in * ; try omega ;
+  rewrite Hbuff in Hbuff2 ; destruct buff2 ; simpl in * ; solve [
+    omega | reflexivity
+  ].
+Qed.
+
+Next Obligation.
+Proof.
+  destruct (Buffer.length (prefix lvli) ≥ 4).
+  + destruct pi ; simpl in H4 |- *; solve [ omega | reflexivity ].
+  + subst. destruct (prefix lvli) ; simpl in * ; solve [ omega | reflexivity ].
+Qed.
+
+Next Obligation.
+Proof.
+  destruct pi0, si; simpl in H1, H3 ; first [
+    discriminate H1 | discriminate H3 | idtac
+  ] ; simpl ; reflexivity.
+Qed.
+
+Program Definition no_buffer_case {A : Set}
+  (lvli : t A)
+  (lvlSi : t (A * A))
+  (Colori : color lvli false = Red)
+  (ColorSi : color lvlSi true <> Red)
+  (Hi : Buffer.length (prefix lvli) <= 1 /\ Buffer.length (suffix lvli) <= 1)
+  (HSi : (Buffer.length (prefix lvlSi)) + (Buffer.length (suffix lvlSi)) <= 1)
+: { b : t A | color b true = Green }
+:=
+  let pi_sig : {
+      b : Buffer.t A | Buffer.length b = 2 + Buffer.length (prefix lvli)
+    }
+  :=
+    match Buffer.length (prefix lvlSi), Buffer.length (suffix lvlSi) with
+    | 1, 0 =>
+      let (pair, _) := Buffer.pop (prefix lvlSi) in
+      let '((elt1, elt2), _) := pair in
+      let (tmpi, _) := Buffer.inject elt1 (prefix lvli) in
+      let (pi, _) := Buffer.inject elt2 tmpi in
+      pi
+    | 0, 1 =>
+      let (pair, _) := Buffer.pop (suffix lvlSi) in
+      let '((elt1, elt2), _) := pair in
+      let (tmpi, _) := Buffer.inject elt1 (prefix lvli) in
+      let (pi, _) := Buffer.inject elt2 tmpi in
+      pi
+    | _, _ => ! (* by HSi *)
+    end
+  in
+  let (pi, Hpi) := pi_sig in
+  let pi_sig2 : { b : Buffer.t A | Buffer.color b = Green } :=
+    match Buffer.length (suffix lvli) with
+    | 0 => pi
+    | 1 =>
+      let (pair, _) := Buffer.pop (suffix lvli) in
+      let (elt, _) := pair in
+      let (pi, _) := Buffer.inject elt pi in
+      pi
+    | _ => !
+    end
+  in
+  let (pi, Hpi) := pi_sig2 in
+  makeLvl pi Buffer.Zero.
+
+Next Obligation.
+Proof.
+  destruct (prefix lvli) ; simpl in H0 ; try omega ; simpl ;
+    [ (right ; trivial) | (left ; discriminate) ].
+Qed.
+
+Next Obligation.
+Proof.
+  left ; destruct (Buffer.length (prefix lvli)) ; try omega ;
+  destruct tmpi ; simpl in H0 ; try omega ;
+  simpl ; discriminate.
+Qed.
+
+Next Obligation.
+Proof.
+  destruct (prefix lvli) ; simpl in H0 ; try omega ; simpl ;
+    [ (right ; trivial) | (left ; discriminate) ].
+Qed.
+
+Next Obligation.
+Proof.
+  left ; destruct (Buffer.length (prefix lvli)) ; try omega ;
+  destruct tmpi ; simpl in H0 ; try omega ;
+  simpl ; discriminate.
+Qed.
+
+Next Obligation.
+Proof.
+  destruct lvlSi; destruct prefix0, suffix0; simpl in *; try omega;
+  contradict ColorSi ; simpl ; reflexivity.
+Qed.
+
+Next Obligation.
+Proof.
+  destruct pi ; simpl in * ; reflexivity || omega.
+Qed.
+
+Next Obligation.
+Proof.
+  left ; destruct pi ; simpl in * ; try omega ; discriminate.
+Qed.
+
+Next Obligation.
+Proof.
+  destruct pi0 ; simpl in * ; first [ reflexivity | omega | idtac ].
+  destruct lvli ; destruct prefix0, suffix0 ; simpl in * ; try omega.
+  simpl in Colori ; discriminate Colori.
+Qed.
+
+Program Definition equilibrate {A : Set} (lvli : t A) (lvlSi : t (A * A))
+  (is_lasti is_lastSi : bool)
+  (Colori : color lvli is_lasti = Red)
+  (ColorSi : color lvlSi is_lastSi <> Red \/ is_empty lvlSi)
+  (Last : is_empty lvlSi -> is_lasti = true)
+  (Triviality : is_lasti = true -> is_lastSi = true)
+  (Has_elements : ~ (is_empty lvli /\ is_empty lvlSi))
+: (
+    { lvl : t A | color lvl false = Green } *
+    { lSi : t (A * A)
+        | color lSi is_lastSi = Red ->
+            color lvlSi is_lastSi <> Green \/ is_lastSi = true
+    }
+  ) +
+  ( 
+    { l : t A | color l true = Green /\ is_lastSi = true }
+  )
+:=
+  match Buffer.length (prefix lvlSi) + Buffer.length (suffix lvlSi) ≥ 2 with
+  | left H => inl (two_buffer_case lvli lvlSi Colori is_lastSi _ _)
+  | right _ =>
+    match Buffer.length (prefix lvli) ≥ 2, Buffer.length (suffix lvli) ≥ 2 with
+    | left _, _
+    | _, left _ =>
+      let '(lvli_sig, lvlSi) :=
+        one_buffer_case lvli lvlSi is_lasti is_lastSi Colori ColorSi _ _ _ _
+      in
+      let (lvli, Hlvli) := lvli_sig in
+      inl (lvli, lvlSi)
+    | right _, right _ =>
+      let (lvli, Hlvli) := no_buffer_case lvli lvlSi Colori _ _ _ in
+      inr lvli
+    end
+  end.
+
+Next Obligation.
+Proof.
+  destruct lvli, is_lasti ; destruct prefix0, suffix0 ;
+  compute in Colori |- *; solve [ discriminate Colori | reflexivity ].
+Qed.
+
+Next Obligation.
+Proof.
+  destruct ColorSi.
+  + assumption.
+  + unfold is_empty in H0 ; rewrite <- 2 Buffer.empty_length in H0.
+    omega.
+Qed.
+
+Next Obligation.
+Proof.
+  clear Heq_anonymous2.
+  left ; simpl in *.
+  destruct lvlSi ; destruct prefix0, suffix0, is_lastSi ; simpl in * ; solve [
+    omega |
+    (compute ; discriminate)
+  ].
+Qed.
+
+Next Obligation.
+Proof.
+  clear Heq_anonymous2.
+  left ; simpl in *.
+  destruct lvlSi ; destruct prefix0, suffix0, is_lastSi ; simpl in * ; solve [
+    omega |
+    (compute ; discriminate)
+  ].
+Qed.
+
+Next Obligation.
+Proof.
+  destruct lvli, is_lasti ; destruct prefix0, suffix0 ;
+  compute in Colori |- *; solve [ discriminate Colori | reflexivity ].
+Qed.
+
+Next Obligation.
+Proof.
+  destruct lvlSi eqn:Si ; destruct prefix0, suffix0 ; simpl in * ; try omega.
+  - assert (H : is_empty lvlSi) by (subst ; compute ; tauto).
+    subst ; apply Last in H.
+    destruct lvli ; simpl in H ; subst ; destruct prefix0, suffix0 ;
+    simpl in * ; try omega ; solve [
+      (contradict Has_elements ; compute ; tauto) |
+      (contradict Colori ; compute ; discriminate)
+    ].
+  - destruct is_lastSi.
+    + compute ; discriminate.
+    + destruct ColorSi as [ Hcolor_fail | Hempty_fail ].
+      * contradict Hcolor_fail ; compute ; reflexivity.
+      * contradict Hempty_fail ; compute ; firstorder.
+  - destruct is_lastSi.
+    + compute ; discriminate.
+    + destruct ColorSi as [ Hcolor_fail | Hempty_fail ].
+      * contradict Hcolor_fail ; compute ; reflexivity.
+      * contradict Hempty_fail ; compute ; firstorder.
+Qed.
+
+Next Obligation.
+Proof.
+  split ; auto.
+  destruct lvlSi, is_lastSi ; destruct prefix0, suffix0 ; simpl in * ;
+  try solve [
+    omega |
+    reflexivity |
+    (compute in ColorSi ; destruct ColorSi as [ Hfalse | Hfalse ] ; [
+        (exfalso ; apply Hfalse ; reflexivity) |
+        (apply Triviality ; apply Last ; compute ; tauto)
+      ])
+  ].
+Qed.
