first_structure/Stack.v
@@ -1,0 +1,55 @@
+Require Import Program.
+
+Require Import Misc.
+Require Level.
+
+Inductive t : Set -> Set -> Type :=
+  | Nil  : forall A, t A A
+  | Cons : forall A B, Level.t A -> t (A * A) B -> t A B.
+
+Arguments Nil [A].
+Arguments Cons [A] [B] _ _.
+
+Fixpoint all_yellows {A B : Set} (s : t A B) (is_last : bool): Prop :=
+  match s with
+  | Nil _ => True
+  | Cons _ _ lvl (Nil _) => Level.color lvl is_last = Yellow
+  | Cons _ _ lvl rest =>
+    Level.color lvl false = Yellow /\ all_yellows rest is_last
+  end.
+
+Definition well_formed {A B : Set} (stack : t A B) is_last :=
+  match stack with
+  | Nil _ => False
+  | Cons _ _ _top_level rest => all_yellows rest is_last
+  end.
+
+Definition is_empty {A B : Set} (stack : t A B) : Prop :=
+  match stack with
+  | Nil _ => True
+  | Cons _ _ lvl (Nil _) => Level.is_empty lvl
+  | _ => False
+  end.
+
+Definition dec_is_empty {A B} (s : t A B) : { is_empty s } + { ~ is_empty s }.
+Proof.
+  destruct s.
+  + left ; simpl ; trivial.
+  + dependent destruction s ; simpl.
+    - apply Level.dec_is_empty.
+    - right ; auto.
+Qed.
+
+Program Definition empty (A : Set) :
+  { s : t A (A * A) | well_formed s false /\ is_empty s } :=
+  Cons (Level.empty A) Nil.
+
+Next Obligation.
+Proof. compute ; tauto. Qed.
+
+Definition color {A B} (s : t A B) b :=
+  match s with
+  | Nil _ => Red
+  | Cons _ _ lvl (Nil _) => Level.color lvl b
+  | Cons _ _ lvl _ => Level.color lvl false
+  end.
